renaming: rename MatchX into CaseX

theories/TM/Code/CaseFin.v
@@ -2,12 +2,12 @@
 
 Require Import ProgrammingTools.
 
-Section MatchFin.
+Section CaseFin.
 
   Variable sig : finType.
   Hypothesis defSig : inhabitedC sig.
 
-  Definition MatchFin : pTM sig^+ sig 1 :=
+  Definition CaseFin : pTM sig^+ sig 1 :=
     Move R;;
     Match (ReadChar)
     (fun s => match s with
@@ -18,13 +18,13 @@ Section MatchFin.
   (** Note that [Encode_Finite] is not globally declared as an instance, because that would cause ambiguity. For example, [bool+bool] is finite, but we might want to encode it with [Encode_sum Encode_bool Encode_bool]. *)
   Local Existing Instance Encode_Finite.
 
-  Definition MatchFin_Rel : pRel sig^+ sig 1 :=
+  Definition CaseFin_Rel : pRel sig^+ sig 1 :=
     fun tin '(yout, tout) => forall x : sig, tin[@Fin0] ≃ x -> isRight tout[@Fin0] /\ yout = x.
 
-  Lemma MatchFin_Sem : MatchFin ⊨c(5) MatchFin_Rel.
+  Lemma CaseFin_Sem : CaseFin ⊨c(5) CaseFin_Rel.
   Proof.
     eapply RealiseIn_monotone.
-    { unfold MatchFin. TM_Correct. }
+    { unfold CaseFin. TM_Correct. }
     { Unshelve. 4,8:reflexivity. all:omega. }
     {
       intros tin (yout, tout) H. intros x HEncX.
@@ -35,19 +35,19 @@ Section MatchFin.
 
   (** There is no need for a constructor, just use [WriteValue] *)
 
-End MatchFin.
+End CaseFin.
 
 
-Arguments MatchFin : simpl never.
-Arguments MatchFin sig {_}. (** Default element is infered and inserted automatically *)
+Arguments CaseFin : simpl never.
+Arguments CaseFin sig {_}. (** Default element is infered and inserted automatically *)
 
 
 
-Ltac smpl_TM_MatchFin :=
+Ltac smpl_TM_CaseFin :=
   lazymatch goal with
-  | [ |- MatchFin _ ⊨ _ ] => eapply RealiseIn_Realise; apply MatchFin_Sem
-  | [ |- MatchFin _ ⊨c(_) _ ] => apply MatchFin_Sem
-  | [ |- projT1 (MatchFin _) ↓ _ ] => eapply RealiseIn_TerminatesIn; apply MatchFin_Sem
+  | [ |- CaseFin _ ⊨ _ ] => eapply RealiseIn_Realise; apply CaseFin_Sem
+  | [ |- CaseFin _ ⊨c(_) _ ] => apply CaseFin_Sem
+  | [ |- projT1 (CaseFin _) ↓ _ ] => eapply RealiseIn_TerminatesIn; apply CaseFin_Sem
   end.
 
-Smpl Add smpl_TM_MatchFin : TM_Correct.
+Smpl Add smpl_TM_CaseFin : TM_Correct.
